\documentclass[24 pt]{article}
\usepackage[cp1250]{inputenc}
\usepackage[T1]{fontenc}
\usepackage{amsmath}
\usepackage{amssymb}
\pagestyle{empty}
\begin{document}
\begin{enumerate}
\renewcommand{\labelenumi}{\alph{enumi})}
\item
\begin{equation*}
\begin{cases}
5x-2y=12\\
-2x-3y=-1\\
\end{cases}
\end{equation*}
\item
\begin{equation*}
\begin{cases}
9x-2y=-64\\
-9x+3y=60\\
\end{cases}
\end{equation*}
\item
\begin{equation*}
\begin{cases}
-4x+5y=31\\
-5x+5y=40\\
\end{cases}
\end{equation*}
\item
\begin{equation*}
\begin{cases}
-4x+8y=8\\
-5x+2y=18\\
\end{cases}
\end{equation*}
\item
\begin{equation*}
\begin{cases}
-5x-6y=-68\\
-9x+y=-28\\
\end{cases}
\end{equation*}
\item
\begin{equation*}
\begin{cases}
-5x+8y=67\\
-7x-8y=17\\
\end{cases}
\end{equation*}
\item
\begin{equation*}
\begin{cases}
-6x+y=-9\\
-4x+9y=19\\
\end{cases}
\end{equation*}
\item
\begin{equation*}
\begin{cases}
4x-y=-43\\
5x-6y=-87\\
\end{cases}
\end{equation*}
\item
\begin{equation*}
\begin{cases}
-x+4y=28\\
4x-9y=-70\\
\end{cases}
\end{equation*}
\item
\begin{equation*}
\begin{cases}
-8x-6y=-58\\
-4x+3y=13\\
\end{cases}
\end{equation*}
\item
\begin{equation*}
\begin{cases}
-3x-7y=-48\\
-7x+6y=22\\
\end{cases}
\end{equation*}
\item
\begin{equation*}
\begin{cases}
-7x+8y=65\\
-4x+6y=40\\
\end{cases}
\end{equation*}
\item
\begin{equation*}
\begin{cases}
9x-4y=-6\\
-x-5y=-32\\
\end{cases}
\end{equation*}
\item
\begin{equation*}
\begin{cases}
-2x-6y=30\\
-6x-2y=-22\\
\end{cases}
\end{equation*}
\item
\begin{equation*}
\begin{cases}
6x-5y=-6\\
-9x-8y=-84\\
\end{cases}
\end{equation*}
\item
\begin{equation*}
\begin{cases}
-9x-9y=-90\\
-2x+2y=-12\\
\end{cases}
\end{equation*}
\item
\begin{equation*}
\begin{cases}
8x+7y=25\\
2x+9y=57\\
\end{cases}
\end{equation*}
\item
\begin{equation*}
\begin{cases}
-6x-3y=21\\
-x-9y=12\\
\end{cases}
\end{equation*}
\item
\begin{equation*}
\begin{cases}
8x+3y=-51\\
-2x-8y=78\\
\end{cases}
\end{equation*}
\item
\begin{equation*}
\begin{cases}
x-7y=-32\\
-9x+4y=-7\\
\end{cases}
\end{equation*}
\item
\begin{equation*}
\begin{cases}
-4x+3y=30\\
5x-2y=-34\\
\end{cases}
\end{equation*}
\item
\begin{equation*}
\begin{cases}
-9x-3y=48\\
4x+3y=-13\\
\end{cases}
\end{equation*}
\item
\begin{equation*}
\begin{cases}
-4x+y=37\\
-7x-4y=59\\
\end{cases}
\end{equation*}
\item
\begin{equation*}
\begin{cases}
5x-2y=-35\\
x-y=-4\\
\end{cases}
\end{equation*}
\item
\begin{equation*}
\begin{cases}
-4x+7y=-65\\
4x+7y=-33\\
\end{cases}
\end{equation*}
\item
\begin{equation*}
\begin{cases}
2x-7y=37\\
2x+7y=-33\\
\end{cases}
\end{equation*}
\end{enumerate}
\end{document}